pcuic/theories/Typing/PCUICClosedTyp.v
@@ -857,9 +857,9 @@ Lemma term_closedn_list_ind :
     (forall k (n : aname) (t : term),
         P k t -> forall t0 : term, P k t0 -> forall t1 : term, P (S k) t1 -> P k (tLetIn n t t0 t1)) ->
     (forall k (t u : term), P k t -> P k u -> P k (tApp t u)) ->
-    (forall k s (u : list Level.t), P  k (tConst s u)) ->
-    (forall k (i : inductive) (u : list Level.t), P k (tInd i u)) ->
-    (forall k (i : inductive) (n : nat) (u : list Level.t), P k (tConstruct i n u)) ->
+    (forall k s (u : Instance.t), P  k (tConst s u)) ->
+    (forall k (i : inductive) (u : Instance.t), P k (tInd i u)) ->
+    (forall k (i : inductive) (n : nat) (u : Instance.t), P k (tConstruct i n u)) ->
     (forall k (ci : case_info) (p : predicate term),
         tCasePredProp_k P k p ->
         forall t0 : term, P k t0 -> forall l : list (branch term),
@@ -975,9 +975,9 @@ Lemma term_noccur_between_list_ind :
     (forall k n (na : aname) (t : term),
         P k n t -> forall t0 : term, P k n t0 -> forall t1 : term, P (S k) n t1 -> P k n (tLetIn na t t0 t1)) ->
     (forall k n (t u : term), P k n t -> P k n u -> P k n (tApp t u)) ->
-    (forall k n s (u : list Level.t), P k n (tConst s u)) ->
-    (forall k n (i : inductive) (u : list Level.t), P k n (tInd i u)) ->
-    (forall k n (i : inductive) (c : nat) (u : list Level.t), P k n (tConstruct i c u)) ->
+    (forall k n s (u : Instance.t), P k n (tConst s u)) ->
+    (forall k n (i : inductive) (u : Instance.t), P k n (tInd i u)) ->
+    (forall k n (i : inductive) (c : nat) (u : Instance.t), P k n (tConstruct i c u)) ->
     (forall k n (ci : case_info) (p : predicate term),
         tCasePredProp_k (fun k' => P k' n) k p -> forall t0 : term, P k n t0 ->
         forall l : list (branch term),
