pcuic/theories/utils/PCUICPretty.v
@@ -202,25 +202,25 @@ Module PrintTermTree.
                         print_term (na' :: Γ) true false body)
     | tApp f l =>
       parens (top || inapp) (print_term Γ false true f ^ " " ^ print_term Γ false false l)
-    | tConst c u => string_of_kername c ^ print_universe_instance u
+    | tConst c u => string_of_kername c ^ print_instance u
     | tInd (mkInd i k) u =>
       match lookup_ind_decl Σ i k with
-      | Some (_, oib) => oib.(ind_name) ^ print_universe_instance u
+      | Some (_, oib) => oib.(ind_name) ^ print_instance u
       | None =>
-        "UnboundInd(" ^ string_of_inductive (mkInd i k) ^ "," ^ string_of_universe_instance u ^ ")"
+        "UnboundInd(" ^ string_of_inductive (mkInd i k) ^ "," ^ string_of_instance u ^ ")"
       end
     | tConstruct (mkInd i k as ind) l u =>
       match lookup_ind_decl Σ i k with
       | Some (_, oib) =>
         match nth_error oib.(ind_ctors) l with
-        | Some cdecl => cdecl.(cstr_name) ^ print_universe_instance u
+        | Some cdecl => cdecl.(cstr_name) ^ print_instance u
         | None =>
           "UnboundConstruct(" ^ string_of_inductive ind ^ "," ^ string_of_nat l ^ ","
-                              ^ string_of_universe_instance u ^ ")"
+                              ^ string_of_instance u ^ ")"
         end
       | None =>
         "UnboundConstruct(" ^ string_of_inductive ind ^ "," ^ string_of_nat l ^ ","
-                            ^ string_of_universe_instance u ^ ")"
+                            ^ string_of_instance u ^ ")"
       end
     | tCase {| ci_ind := mkInd mind i as ind; ci_npar := pars |} p t brs =>
       match lookup_ind_decl Σ mind i with
